src/OeufProof.v
@@ -16,8 +16,10 @@ Require ElimFuncComp2.
 Require ElimFuncComp3.
 Require SwitchedComp.
 Require SelfCloseComp.
-Require SelfNumberedComp.
-Require FlattenedComp.
+Require StackCompCombined.
+Require LocalsCompCombined.
+Require FlatCompCombined.
+Require FmajorComp.
 Require Fmajortofflatmajor.
 Require Fflatmajortoemajor.
 Require Emajortodmajor.
@@ -42,6 +44,32 @@ Require Import EricTact.
 
 (* Theorem: given 2 x86 level values and their matching high level values, we can build a call out of them and establish matching with it *)
 
+Ltac break_result_chain :=
+    let go l :=
+        match l with
+        | OK _ => fail 1
+        | _ => destruct l eqn:?; try discriminate
+        end in
+    repeat match goal with
+    | [ H : context [ ?l @@ ?r ] |- _ ] => go l
+    | [ H : context [ ?l @@@ ?r ] |- _ ] => go l
+    end.
+
+Ltac break_result_chain' :=
+    repeat match goal with
+    | [ H : context [ OK ?l @@ ?r ] |- _ ] => unfold Compiler.apply_total in H at 1
+    | [ H : context [ OK ?l @@@ ?r ] |- _ ] => unfold Compiler.apply_partial in H at 1
+    | [ H : context [ ?l @@ ?r ] |- _ ] => destruct l eqn:?; try discriminate
+    | [ H : context [ ?l @@@ ?r ] |- _ ] => destruct l eqn:?; try discriminate
+    end.
+
+Ltac inject_ok :=
+    repeat match goal with
+    | [ H : OK ?x = OK ?y |- _ ] =>
+            assert (x = y) by congruence;
+            clear H
+    end.
+
 Section Simulation.
 
   Variable prog : compilation_unit.
@@ -64,9 +92,32 @@ Section Simulation.
 
     (* Break down structure of compiler *)
     unfold transf_untyped_to_asm in *.
-    unfold Compiler.apply_partial in *.
-    repeat (break_match_hyp; try congruence).
     unfold transf_untyped_to_cminor in *.
+    Set Default Timeout 10.
+
+    repeat match goal with
+    | [ H : OK ?l @@ ?r = _ |- _ ] => unfold Compiler.apply_total in H at 1
+    | [ H : OK ?l @@@ ?r = _ |- _ ] => unfold Compiler.apply_partial in H at 1
+    | [ H : ?l @@ ?r = _ |- _ ] => destruct l eqn:?; try discriminate
+    | [ H : ?l @@@ ?r = _ |- _ ] => destruct l eqn:?; try discriminate
+    | [ H : OK ?l = OK ?r |- _ ] =>
+            assert (l = r) by congruence;
+            clear H
+    | [ H : option_to_res ?l = OK ?r |- _ ] =>
+            assert (l = Some r) by
+                (clear -H; unfold option_to_res in H; destruct l; congruence);
+            clear H
+    end.
+
+  (*
+    break_result_chain.
+    unfold Compiler.apply_partial in Heqr0 at 1.
+    unfold Compiler.apply_partial in Heqr at 1.
+    break_result_chain.
+    break_result_chain.
+    unfold Compiler.apply_partial in *.
+
+    repeat (break_match_hyp; try congruence).
     unfold Compiler.apply_partial in *.
     unfold Compiler.apply_total in *.
     repeat (break_match_hyp; try congruence).
@@ -79,13 +130,11 @@ Section Simulation.
            | [ H : OK _ = OK _ |- _ ] => inversion H; clear H
            end.
     subst p16 p17 p18 p20.
+  *)
 
     (* Untyped to Lifted *)
     eapply compose_notrace_mix_forward_simulation.
-    set (p1' := LiftedComp.compile_cu p1).
-
     eapply LiftedComp.fsim; try eassumption.
-    instantiate (1 := p1'). subst p1'. reflexivity.
 
     (* Lifted to Tagged *)
     eapply compose_notrace_mix_forward_simulation.
@@ -117,9 +166,9 @@ Section Simulation.
     eapply compose_notrace_mix_forward_simulation.
     eapply SelfCloseComp.fsim; try eassumption.
 
-    (* SelfClose to SelfNumbered *)
+    (* SelfClose to StackFlatter2 *)
     eapply compose_notrace_mix_forward_simulation.
-    eapply SelfNumberedComp.fsim; try eassumption.
+    eapply StackCompCombined.fsim; try eassumption.
 
     (* SelfNumbered to Flattened *)
     eapply compose_notrace_mix_forward_simulation.
